Proof golf

LeanToLambdaBox/Contexts.lean
@@ -21,17 +21,6 @@ private def weakenId: MultiExtension ctx ctx' -> ctx.Id -> ctx'.Id := Fin.castLE
 end MultiExtension
 end GenericSizedContext
 
-private theorem list_index_cast { l' l: List α } (eq: l' = l) (i: Fin (l.length)): l'[Fin.cast (congrArg List.length eq).symm i] = l[i] := by
-  cases eq
-  rfl
-
-private theorem length_le_length_append {as bs: List α}: as.length ≤ (as ++ bs).length := by
-  rewrite [List.length_append]
-  apply Nat.le_add_right
-
-private theorem getElem_append_left_fin (as bs: List α) (i: Fin as.length) (h: as.length <= (as ++ bs).length): (as ++ bs)[Fin.castLE h i] = as[i] := by
-  apply List.getElem_append_left
-
 private abbrev GenericArrayContext α := Array α
 namespace GenericArrayContext
 private def empty: GenericArrayContext α := Array.empty
@@ -54,18 +43,15 @@ private def weakenId (ext: MultiExtension ctx ctx'): ctx.Id -> ctx'.Id :=
   Fin.castLE (by 
     show ctx.toList.length ≤ ctx'.toList.length
     cases ext with | intro _ h =>
-    rewrite [<-h]
-    exact length_le_length_append
+    rewrite [<-h, List.length_append]
+    apply Nat.le_add_right
   )
 
 private theorem weakenId_getInfo: (@weakenId α ctx ctx' ext i).getInfo = i.getInfo := by
-  let i' := ext.weakenId i
   cases ext with | intro _ h =>
-  show ctx'.toList[i'] = ctx.toList[i]
-  unfold Id Array.size -- unfolding implicit things in the goal, set pp.explicit to suffer
-  rewrite [<-list_index_cast h i']
-  apply getElem_append_left_fin
-  exact length_le_length_append
+  show ctx'.toList.get _  = _
+  rewrite [List.get_of_eq h.symm]
+  apply List.getElem_append_left
 
 end MultiExtension
 end GenericArrayContext
@@ -149,37 +135,31 @@ namespace MultiExtension
 def trivial: MultiExtension ctx ctx := GenericArrayContext.MultiExtension.trivial
 @[irreducible]
 def compose: MultiExtension ctx ctx' -> MultiExtension ctx' ctx'' -> MultiExtension ctx ctx'' := GenericArrayContext.MultiExtension.compose
+
 @[irreducible, local semireducible]
 def weakenMutualInductiveId: MultiExtension ctx ctx' -> ctx.MutualInductiveId -> ctx'.MutualInductiveId := GenericArrayContext.MultiExtension.weakenId
 
-theorem weakenMutualInductiveId_inductiveArities : (@weakenMutualInductiveId ctx ctx' ext mid).inductiveArities = mid.inductiveArities := by
-  unfold MutualInductiveId.inductiveArities
-  apply congrArg
-  apply GenericArrayContext.MultiExtension.weakenId_getInfo
+unseal MutualInductiveId.inductiveArities
+theorem weakenMutualInductiveId_inductiveArities : (@weakenMutualInductiveId ctx ctx' ext mid).inductiveArities = mid.inductiveArities :=
+  congrArg (MutualInductiveSpec.arities) GenericArrayContext.MultiExtension.weakenId_getInfo
 
 unseal InductiveId
-
 @[irreducible, local semireducible]
 def weakenInductiveId (ext: MultiExtension ctx ctx') (iid: @InductiveId ctx mid): (ext.weakenMutualInductiveId mid).InductiveId :=
   Fin.cast (congrArg List.length weakenMutualInductiveId_inductiveArities).symm iid
 
-theorem weakenInductiveId_constructorArities: (@weakenInductiveId ctx ctx' mid ext iid).constructorArities = iid.constructorArities := by
-  unfold MutualInductiveId.InductiveId.constructorArities
-  unfold InductiveId at iid
-  show (ext.weakenMutualInductiveId mid).inductiveArities[show Fin _ from ext.weakenInductiveId iid] = mid.inductiveArities[iid]
-  exact (list_index_cast weakenMutualInductiveId_inductiveArities iid)
-
+unseal MutualInductiveId.InductiveId.constructorArities
+theorem weakenInductiveId_constructorArities: (@weakenInductiveId ctx ctx' mid ext iid).constructorArities = iid.constructorArities :=
+  List.get_of_eq weakenMutualInductiveId_inductiveArities _
 
 unseal ConstructorId
 @[irreducible, local semireducible]
 def weakenConstructorId (ext: MultiExtension ctx ctx') (cid: @ConstructorId ctx mid iid): (ext.weakenInductiveId iid).ConstructorId :=
   Fin.cast (congrArg List.length weakenInductiveId_constructorArities).symm cid
 
-theorem weakenConstructorId_arity: (@weakenConstructorId ctx ctx' mid iid ext cid).arity = cid.arity := by
-  unfold MutualInductiveId.InductiveId.ConstructorId.arity
-  unfold ConstructorId at cid
-  show (ext.weakenInductiveId iid).constructorArities[show Fin _ from ext.weakenConstructorId cid] = iid.constructorArities[cid]
-  exact (list_index_cast weakenInductiveId_constructorArities cid)
+unseal MutualInductiveId.InductiveId.ConstructorId.arity
+theorem weakenConstructorId_arity: (@weakenConstructorId ctx ctx' mid iid ext cid).arity = cid.arity :=
+  List.get_of_eq weakenInductiveId_constructorArities _
 
 end MultiExtension
 end InductiveContext
